coq: Add basic error reporting to the typechecking phase

Syntax.v
@@ -4,13 +4,14 @@ Inductive Port :=
   P0 | P1.
 
 Section Syntax.
-  Context {var_t reg_t fn_t: Type}.
+  Context {pos_t var_t reg_t fn_t: Type}.
 
   Inductive uexpr :=
   | UVar (var: var_t)
   | UConst {n} (cst: bits n)
   | URead (port: Port) (idx: reg_t)
-  | UCall (fn: fn_t) (arg1: uexpr) (arg2: uexpr).
+  | UCall (fn: fn_t) (arg1: uexpr) (arg2: uexpr)
+  | UEPos (p: pos_t) (e: uexpr).
 
   Inductive urule  :=
   | USkip
@@ -18,11 +19,13 @@ Section Syntax.
   | USeq (r1 r2: urule)
   | UBind (v: var_t) (ex: uexpr) (body: urule)
   | UIf (cond: uexpr) (tbranch: urule) (fbranch: urule)
-  | UWrite (port: Port) (idx: reg_t) (value: uexpr).
+  | UWrite (port: Port) (idx: reg_t) (value: uexpr)
+  | URPos (p: pos_t) (r: urule).
 
   Inductive uscheduler :=
   | UDone
-  | UTry (r: urule) (s1 s2: uscheduler).
+  | UTry (r: urule) (s1 s2: uscheduler)
+  | USPos (p: pos_t) (s: uscheduler).
 End Syntax.
 
 Arguments uexpr : clear implicits.
